src/lang/Thread.v
@@ -17,6 +17,25 @@ Require Import Commit.
 Set Implicit Arguments.
 
 
+Module ThreadEvent.
+  Inductive t :=
+  | silent
+  | promise (loc:Loc.t) (from to:Time.t) (val:Const.t) (released:Capability.t)
+  | read (loc:Loc.t) (ts:Time.t) (val:Const.t) (ord:Ordering.t)
+  | write (loc:Loc.t) (ts:Time.t) (val:Const.t) (ord:Ordering.t)
+  | update (loc:Loc.t) (tsr tsw:Time.t) (valr valw:Const.t) (ordr ordw:Ordering.t)
+  | fence (ordr ordw:Ordering.t)
+  | syscall (e:Event.t)
+  .
+
+  Definition get_event (e:t): option Event.t :=
+    match e with
+    | syscall e => Some e
+    | _ => None
+    end.
+End ThreadEvent.
+
+
 Module Local.
   Structure t := mk {
     commit: Commit.t;
@@ -286,70 +305,71 @@ Module Thread.
       memory: Memory.t;
     }.
 
-    Inductive promise_step (e1:t): forall (e2:t), Prop :=
+    Inductive promise_step (e1:t) loc from to val released: forall (e2:t), Prop :=
     | promise_step_intro
-        loc from to val released lc2 mem2
+        lc2 mem2
         (LOCAL: Local.promise_step e1.(local) e1.(memory) loc from to val released lc2 mem2):
-        promise_step e1 (mk e1.(state) lc2 mem2)
+        promise_step e1 loc from to val released (mk e1.(state) lc2 mem2)
     .
 
-    Inductive program_step: forall (e:option Event.t) (readinfo: option (Loc.t * Time.t)) (e1 e2:t), Prop :=
+    Inductive program_step: forall (e:ThreadEvent.t) (e1 e2:t), Prop :=
     | step_silent
         st1 lc1 mem1
         st2 lc2
         (STATE: lang.(Language.step) None st1 st2)
         (LOCAL: Local.silent_step lc1 mem1 lc2):
-        program_step None None (mk st1 lc1 mem1) (mk st2 lc2 mem1)
+        program_step ThreadEvent.silent (mk st1 lc1 mem1) (mk st2 lc2 mem1)
     | step_read
         st1 lc1 mem1
         st2 loc ts val released ord lc2
-        (STATE: lang.(Language.step) (Some (ThreadEvent.mem (MemEvent.read loc val ord))) st1 st2)
+        (STATE: lang.(Language.step) (Some (ProgramEvent.read loc val ord)) st1 st2)
         (LOCAL: Local.read_step lc1 mem1 loc ts val released ord lc2):
-        program_step None (Some (loc, ts)) (mk st1 lc1 mem1) (mk st2 lc2 mem1)
+        program_step (ThreadEvent.read loc ts val ord) (mk st1 lc1 mem1) (mk st2 lc2 mem1)
     | step_write
         st1 lc1 mem1
         st2 loc from to val released ord lc2 mem2
-        (STATE: lang.(Language.step) (Some (ThreadEvent.mem (MemEvent.write loc val ord))) st1 st2)
+        (STATE: lang.(Language.step) (Some (ProgramEvent.write loc val ord)) st1 st2)
         (LOCAL: Local.write_step lc1 mem1 loc from to val released released ord lc2 mem2):
-        program_step None None (mk st1 lc1 mem1) (mk st2 lc2 mem2)
+        program_step (ThreadEvent.write loc to val ord) (mk st1 lc1 mem1) (mk st2 lc2 mem2)
     | step_update
         st1 lc1 mem1
         st3 loc ordr ordw
         tsr valr releasedr lc2
         tsw valw releasedw lc3 mem3
-        (STATE: lang.(Language.step) (Some (ThreadEvent.mem (MemEvent.update loc valr valw ordr ordw))) st1 st3)
+        (STATE: lang.(Language.step) (Some (ProgramEvent.update loc valr valw ordr ordw)) st1 st3)
         (LOCAL1: Local.read_step lc1 mem1 loc tsr valr releasedr ordr lc2)
         (LOCAL2: Local.write_step lc2 mem1 loc tsr tsw valw releasedw (Capability.join releasedr releasedw) ordw lc3 mem3):
-        program_step None (Some (loc, tsr)) (mk st1 lc1 mem1) (mk st3 lc3 mem3)
+        program_step (ThreadEvent.update loc tsr tsw valr valw ordr ordw) (mk st1 lc1 mem1) (mk st3 lc3 mem3)
     | step_fence
         st1 lc1 mem1
         st2 ordr ordw lc2
-        (STATE: lang.(Language.step) (Some (ThreadEvent.mem (MemEvent.fence ordr ordw))) st1 st2)
+        (STATE: lang.(Language.step) (Some (ProgramEvent.fence ordr ordw)) st1 st2)
         (LOCAL: Local.fence_step lc1 mem1 ordr ordw lc2):
-        program_step None None (mk st1 lc1 mem1) (mk st2 lc2 mem1)
+        program_step (ThreadEvent.fence ordr ordw) (mk st1 lc1 mem1) (mk st2 lc2 mem1)
     | step_syscall
         st1 lc1 mem1
         st2 e lc2
-        (STATE: lang.(Language.step) (Some (ThreadEvent.syscall e)) st1 st2)
+        (STATE: lang.(Language.step) (Some (ProgramEvent.syscall e)) st1 st2)
         (LOCAL: Local.fence_step lc1 mem1 Ordering.seqcst Ordering.seqcst lc2):
-        program_step (Some e) None (mk st1 lc1 mem1) (mk st2 lc2 mem1)
+        program_step (ThreadEvent.syscall e) (mk st1 lc1 mem1) (mk st2 lc2 mem1)
     .
 
-    Inductive step: forall (e:option Event.t) (readinfo:option (Loc.t * Time.t)) (e1 e2:t), Prop :=
+    Inductive step: forall (e:ThreadEvent.t) (e1 e2:t), Prop :=
     | step_promise
-        e1 e2
-        (STEP: promise_step e1 e2):
-        step None None e1 e2
+        loc from to val released e1 e2
+        (STEP: promise_step e1 loc from to val released e2):
+        step (ThreadEvent.promise loc from to val released) e1 e2
     | step_program
-        e readinfo e1 e2
-        (STEP: program_step e readinfo e1 e2):
-        step e readinfo e1 e2
+        e e1 e2
+        (STEP: program_step e e1 e2):
+        step e e1 e2
     .
 
     Inductive tau_step (e1 e2:t): Prop :=
     | step_tau
-        readinfo
-        (STEP: step None readinfo e1 e2)
+        e
+        (STEP: step e e1 e2)
+        (TAU: ThreadEvent.get_event e = None)
     .
 
     Definition consistent st1 lc1 mem: Prop :=
@@ -360,8 +380,9 @@ Module Thread.
         <<STEPS: rtc tau_step (mk st1 lc1 mem1) e2>> /\
         <<PROMISES: e2.(local).(Local.promises) = Memory.bot>>.
 
-    Lemma promise_step_future e1 e2
-          (STEP: promise_step e1 e2)
+    Lemma promise_step_future
+          loc from to val released e1 e2
+          (STEP: promise_step e1 loc from to val released e2)
           (WF1: Local.wf e1.(local) e1.(memory)):
       <<WF2: Local.wf e2.(local) e2.(memory)>> /\
       <<FUTURE: Memory.future e1.(memory) e2.(memory)>>.
@@ -369,8 +390,8 @@ Module Thread.
       inv STEP; s. exploit Local.promise_step_future; eauto.
     Qed.
 
-    Lemma program_step_future e readinfo e1 e2
-          (STEP: program_step e readinfo e1 e2)
+    Lemma program_step_future e e1 e2
+          (STEP: program_step e e1 e2)
           (WF1: Local.wf e1.(local) e1.(memory)):
       <<WF2: Local.wf e2.(local) e2.(memory)>> /\
       <<FUTURE: Memory.future e1.(memory) e2.(memory)>>.
@@ -385,14 +406,14 @@ Module Thread.
       - exploit Local.fence_step_future; eauto. i. splits; ss. refl.
     Qed.
 
-    Lemma step_future e readinfo e1 e2
-          (STEP: step e readinfo e1 e2)
+    Lemma step_future e e1 e2
+          (STEP: step e e1 e2)
           (WF1: Local.wf e1.(local) e1.(memory)):
       <<WF2: Local.wf e2.(local) e2.(memory)>> /\
       <<FUTURE: Memory.future e1.(memory) e2.(memory)>>.
     Proof.
       inv STEP.
-      - apply promise_step_future; auto.
+      - eapply promise_step_future; eauto.
       - eapply program_step_future; eauto.
     Qed.
 
@@ -410,8 +431,9 @@ Module Thread.
         splits; ss. etrans; eauto.
     Qed.
 
-    Lemma promise_step_disjoint e1 e2 lc
-        (STEP: promise_step e1 e2)
+    Lemma promise_step_disjoint
+          loc from to val released e1 e2 lc
+        (STEP: promise_step e1 loc from to val released e2)
         (WF1: Local.wf e1.(local) e1.(memory))
         (DISJOINT1: Local.disjoint e1.(local) lc)
         (WF: Local.wf lc e1.(memory)):
@@ -423,8 +445,8 @@ Module Thread.
       exploit Local.promise_step_disjoint; eauto.
     Qed.
 
-    Lemma program_step_disjoint e readinfo e1 e2 lc
-        (STEP: program_step e readinfo e1 e2)
+    Lemma program_step_disjoint e e1 e2 lc
+        (STEP: program_step e e1 e2)
         (WF1: Local.wf e1.(local) e1.(memory))
         (DISJOINT1: Local.disjoint e1.(local) lc)
         (WF: Local.wf lc e1.(memory)):
@@ -448,8 +470,8 @@ Module Thread.
         exploit Local.fence_step_disjoint; eauto.
     Qed.
 
-    Lemma step_disjoint e readinfo e1 e2 lc
-        (STEP: step e readinfo e1 e2)
+    Lemma step_disjoint e e1 e2 lc
+        (STEP: step e e1 e2)
         (WF1: Local.wf e1.(local) e1.(memory))
         (DISJOINT1: Local.disjoint e1.(local) lc)
         (WF: Local.wf lc e1.(memory)):
